compiler/backend/semantics/stackPropsScript.sml
@@ -466,7 +466,9 @@ val reg_name_def = Define`
   reg_name r c ⇔
   r < c.reg_count - LENGTH (c.avoid_regs)`
 
-(* TODO: for FP *)
+val fp_reg_name_def = Define `
+  fp_reg_name d c ⇔
+  d < c.fp_reg_count`
 
 (* inst requirements just before stack_names *)
 
@@ -505,6 +507,36 @@ val arith_name_def = Define`
     reg_name r3 c ∧ reg_name r4 c ∧
     (c.ISA = MIPS ∨ c.ISA = RISC_V ⇒ r1 ≠ r3))`
 
+(* We could actually almost use fp_ok, except this needs to check reg_ok for
+   some registers as well *)
+val fp_name_def = Define `
+  (fp_name (FPLess r d1 d2) c <=>
+      reg_name r c /\ fp_reg_name d1 c /\ fp_reg_name d2 c) /\
+  (fp_name (FPLessEqual r d1 d2) c <=>
+      reg_name r c /\ fp_reg_name d1 c /\ fp_reg_name d2 c) /\
+  (fp_name (FPEqual r d1 d2) c <=>
+      reg_name r c /\ fp_reg_name d1 c /\ fp_reg_name d2 c) /\
+  (fp_name (FPAbs d1 d2) c <=> fp_reg_name d1 c /\ fp_reg_name d2 c) /\
+  (fp_name (FPNeg d1 d2) c <=> fp_reg_name d1 c /\ fp_reg_name d2 c) /\
+  (fp_name (FPSqrt d1 d2) c <=> fp_reg_name d1 c /\ fp_reg_name d2 c) /\
+  (fp_name (FPAdd d1 d2 d3) c <=>
+      fp_reg_name d1 c /\ fp_reg_name d2 c /\ fp_reg_name d3 c) /\
+  (fp_name (FPSub d1 d2 d3) c <=>
+      fp_reg_name d1 c /\ fp_reg_name d2 c /\ fp_reg_name d3 c) /\
+  (fp_name (FPMul d1 d2 d3) c <=>
+      fp_reg_name d1 c /\ fp_reg_name d2 c /\ fp_reg_name d3 c) /\
+  (fp_name (FPDiv d1 d2 d3) c <=>
+      fp_reg_name d1 c /\ fp_reg_name d2 c /\ fp_reg_name d3 c) /\
+  (fp_name (FPMov d1 d2) c <=> fp_reg_name d1 c /\ fp_reg_name d2 c) /\
+  (fp_name (FPMovToReg r1 r2 d) (c : 'a asm_config) <=>
+      reg_name r1 c /\ ((dimindex(:'a) = 32) ==> r1 <> r2 /\ reg_name r2 c) /\
+      fp_reg_name d c) /\
+  (fp_name (FPToInt r d) c <=> reg_name r c /\ fp_reg_name d c) /\
+  (fp_name (FPMovFromReg d r1 r2) (c : 'a asm_config) <=>
+      reg_name r1 c /\ ((dimindex(:'a) = 32) ==> r1 <> r2 /\ reg_name r2 c) /\
+      fp_reg_name d c) /\
+  (fp_name (FPFromInt d r) c <=> reg_name r c /\ fp_reg_name d c)`
+
 val addr_name_def = Define`
   addr_name m (Addr r w) c ⇔
   reg_name r c ∧
@@ -514,6 +546,7 @@ val inst_name_def = Define`
   (inst_name c (Const r w) ⇔ reg_name r c) ∧
   (inst_name c (Mem m r a) ⇔ reg_name r c ∧ addr_name m a c) ∧
   (inst_name c (Arith x) ⇔ arith_name x c) ∧
+  (inst_name c (FP f) ⇔ fp_name f c) ∧
   (inst_name _ _ = T)`
 
 val stack_asm_name_def = Define`
